Duplicate of Shamila's commit in the feval_decomp branch with one renaming and one modified branch (when the head isn't the element we're looking for). Applied Shamila's function to feval.
Also some trivial cases in the proof of feval_sound have been handled.

FEV_Definitions.v
@@ -26,25 +26,18 @@ Notation fbenv := (list (var * fexp)).
 Notation fmths := (list (mname * (typ * env * fexp))).
 Notation fctable := (list (cname * (cname * flds * fmths))).
 
-Fixpoint getrm {A:Type} (x: atom) (E: list (atom * A)) : option (A * (list (atom * A))) :=
-  match E with
+(* Assumes an ordering such that parents are closer to the nil in fct *)
+Fixpoint fmbody (cn:cname) (mn:mname) (fct:fctable) : option (env * fexp) :=
+  match fct with
+  | (C,(D,_,ms))::t =>
+    if C == cn then
+      match get mn ms with
+      | Some (_, en, ex) => Some (en, ex)
+      | None => fmbody D mn t
+      end
+    else fmbody cn mn t
   | nil => None
-  | (y,v)::E => if x == y then Some (v, E) else
-    match getrm x E with
-    | Some (v', E') => Some (v', (y,v)::E')
-    | None => None
-    end
   end.
-
-(*Fixpoint fmbody (cn:cname) (mn:mname) (fct:fctable) : option (env * fexp) :=
-  match getrm cn fct with
-  | Some ((pn, _, ms), fctr) =>
-    match get mn ms with
-    | Some (_, en, ex) => Some (en, ex) (* Method found for class *)
-    | None => fmbody pn mn fctr (* Recursive call to find in parent classes *)
-    end
-  | None => None (* Class not found *)
-  end.*)
 
 Fixpoint subst_fexp (E : fbenv) (e : fexp) {struct e} : fexp :=
     match e with
@@ -82,13 +75,9 @@ Fixpoint feval (e:fexp) (fct:fctable) : option fexp :=
             | (emb, emps) =>
               match emb with
               | f_new cn =>
-                match get cn fct with
-                | Some (_, _, ms) =>
-                  match get mn ms with
-                  | Some (_, en, ex) => Some (subst_fexp ((this, em)::(combine (List.map fst en) ps)) ex) (* R-INVK *)
-                  | None => None (* TODO: Case for inheritance *)
-                  end
-                | None => None (* Class not found *)
+                match fmbody cn mn fct with
+                | Some (en, ex) => Some (subst_fexp ((this, em)::(combine (List.map fst en) ps)) ex) (* R-INVK *)
+                | None => None (* No such method in the hierarchy *)
                 end
               | emb => None (* Method call on application to non-object *)
               end
